added some files

IntStable.fst
@@ -5,47 +5,86 @@
 module IntStable
 open FStar.List.Tot
 open FStar.ListProperties
+open IntSort
 (*
   This module is heavily inspired by Leino and Lucio's 2012 paper,
   'An Assertional Proof of the Stability and Correctness of Natural Mergesort'.
   http://research.microsoft.com/en-us/um/people/leino/papers/krml241.pdf
 *)
 
+val appears_before: before:int -> after:int -> ls: list int -> Tot bool
+let rec appears_before b4 aft ls =
+  match ls with
+  | _ | [_] -> false
+  | hd::tl ->
+    if hd = b4 then mem aft tl
+    else appears_before b4 aft tl
+
+type stable (l1:list int) (l2:list int{permutation l1 l2}) =
+  forall x y. ((appears_before x y l1 /\ x = y) ==> appears_before x y l2)
+
 (**
   filterEq returns the elements of a list that have the same key as n.
 **)
-val filterEq: (n: int) -> (xs: list int) -> Tot (list int)
-let rec filterEq n xs =
+val filter_eq: (n: int) -> (xs: list int) -> Tot (list int)
+let rec filter_eq n xs =
   match xs with
   | [] -> []
   | hd::tl
     -> if n = hd then
-        Cons hd (filterEq n tl)
-      else filterEq n tl
+        Cons hd (filter_eq n tl)
+      else filter_eq n tl
 
 (**
-  The stability predicate
+  Ensures that filtering is distinct with regards to append.
 **)
-type stable (xs: list int) (ys:list int) = forall x. filterEq x xs = filterEq x ys
-
-(**
-  Ensures that filtering is distinct with regards to append
-**)
-val distFilterApp: (x: int) -> (xs: list int) -> (ys: list int) ->
+val dist_filter_app: (x: int) -> (xs: list int) -> (ys: list int) ->
   Lemma
-  (ensures (filterEq x (append xs ys) = append (filterEq x xs) (filterEq x ys)))
-let rec distFilterApp x xs ys =
+  (ensures (filter_eq x (append xs ys) = append (filter_eq x xs) (filter_eq x ys)))
+let rec dist_filter_app x xs ys =
   match xs with
   | [] | [_] -> (match ys with
     | [] | [_] -> ()
-    | a::b::cs -> distFilterApp x xs (Cons b cs))
-  | a::b::cs -> distFilterApp x (Cons b cs) ys
+    | a::b::cs -> dist_filter_app x xs (Cons b cs))
+  | a::b::cs -> dist_filter_app x (Cons b cs) ys
 
-val nullFilter: (x:int) -> (ys: list int) ->
+(**
+  Ensures that if a key does not appear in a list, then filtering for it returns [].
+**)
+val null_filter: (x:int) -> (ys: list int) ->
   Lemma
   (requires not (mem x ys))
-  (ensures filterEq x ys = [])
-let rec nullFilter x ys =
+  (ensures filter_eq x ys = [])
+let rec null_filter x ys =
   match ys with
   | [] | [_] -> ()
-  | a::b::cs -> nullFilter x (Cons b cs)
+  | a::b::cs -> null_filter x (Cons b cs)
+
+(*
+val stable_lifting: (x:int)
+  -> (ws:list int{is_Cons ws})
+  -> (zs:list int{sorted zs /\ is_Cons zs})
+  -> Lemma (requires Cons.hd ws < Cons.hd zs /\ x = Cons.hd ws)
+  (ensures (stable (zs@ws) ((Cons (Cons.hd ws) zs)@(Cons.tl ws))))
+let stable_lifting x ws zs =
+  dist_filter_app x zs ws;
+  //assert(filter_eq x (zs@ws) = (filter_eq x zs)@(filter_eq x ws));
+  //assert((filter_eq x zs)@((filter_eq x (Cons (Cons.hd ws) [])@(filter_eq x (Cons.tl ws)))) = filter_eq x (zs@ws));
+  append_assoc (filter_eq x zs) (filter_eq x (Cons (Cons.hd ws) [])) (filter_eq x (Cons.tl ws));
+  //assert((((filter_eq x zs)@(filter_eq x (Cons (Cons.hd ws) [])))@(filter_eq x (Cons.tl ws))) = filter_eq x (zs@ws));
+  if (x = Cons.hd ws) then (
+    null_filter x zs;
+    append_nil_l (Cons (Cons.hd ws) []);
+    append_l_nil (Cons (Cons.hd ws) []);
+    dist_filter_app x (Cons (Cons.hd ws) []) (Cons.tl ws))
+    //assert((filter_eq x (zs@ws)) = (filter_eq x ((Cons (Cons.hd ws) zs))@(Cons.tl ws)));
+    //assert((filter_eq x (zs@ws)) = (filter_eq x (Cons (Cons.hd ws) (zs@(Cons.tl ws))))))
+
+  else (append_l_nil (filter_eq x zs);
+    assert(filter_eq x (Cons (Cons.hd ws) []) = []);
+    append_nil_l zs;
+    append_l_nil zs;
+    dist_filter_app x zs (Cons.tl ws))
+    //assert((filter_eq x (zs@ws)) = (filter_eq x ((Cons (Cons.hd ws) zs))@(Cons.tl ws)));
+    //assert((filter_eq x (zs@ws)) <> (filter_eq x (Cons (Cons.hd ws) (zs@(Cons.tl ws))))))
+*)
