MergeSort.fst
@@ -1,22 +1,89 @@
 module MergeSort
 open FStar.List.Tot
-open IntSort
+open GenericSort
+open GenericStability
 
-type split_inv (l:list int) (l1:list int) (l2:list int) =
+val merge: #a:eqtype
+  -> l_0:list a{is_Cons l_0}
+  -> l_1:list a{is_Cons l_1}
+  -> key:(a -> Tot int){sorted l_0 key /\ sorted l_1 key}
+  -> l':list a{sorted l' key /\ permutation_2 l' l_0 l_1}
+
+let rec merge #a l_0 l_1 key =
+  let h_0 = hd l_0 in
+  let h_1 = hd l_1 in
+  if ((key h_0) <= (key h_1)) then
+    if tl l_0 = [] then (h_0::l_1)
+    else
+    (cons_sorted h_0 (merge (tl l_0) l_1 key) key;
+    h_0::(merge (tl l_0) l_1 key))
+  else if tl l_1 = [] then (h_1::l_0)
+    else
+    cons_sorted h_1 (merge l_0 (tl l_1) key) key;
+    h_1::(merge l_0 (tl l_1) key)
+(*)
+  match ((key h_0) <= (key h_1)) with
+  | true ->
+    cons_sorted h_0 (merge (tl l_0) l_1 key) key;
+    h_0::(merge (tl l_0) l_1 key)
+  | false ->
+      cons_sorted h_1 (merge l_0 (tl l_1) key) key;
+      h_1::(merge l_0 (tl l_1) key)
+
+(*)
+val ms: #a:eqtype -> l_0:list a -> key:(a -> Tot int) -> l':list a
+let ms #a l_0 key =
+  match l_0 with
+  | [] | [_] -> l_0
+  | [a_0;a_1] -> (if key a_0 <= key a_1 then [a_0;a_1] else [a_1;a_0])
+  | [a_0;a_1;a_2] -> []
+
+
+
+
+
+
+
+
+
+
+
+
+
+
+
+
+
+
+
+
+
+
+
+
+
+(*)
+type split_inv (#a:eqtype) (l:list a) (l1:list a) (l2:list a) (key:(a -> Tot int)) =
     permutation_2 l l1 l2 /\
     (* needed for decreases clause in mergesort function *)
     length l > length l1 /\ length l > length l2
+    /\ (forall x y.
+    (appears_before x y l ==>
+    appears_before x y l1
+    \/ appears_before x y l2
+    \/ ~(mem x l1 /\ mem y l1 )))
 
-val split: l:list int -> Pure (list int * list int)
-             (requires (is_Cons l /\ is_Cons (Cons.tl l)))
-	     (ensures (fun r -> split_inv l (fst r) (snd r)))
+
+val split: (#a:eqtype) -> l:list a -> Tot r:(list a * list a)
+  (requires (is_Cons l /\ is_Cons (Cons.tl l)))
+	(ensures (split_inv l (fst r) (snd r)))
 let rec split (x::y::l) =
   match l with
     | [] -> [x], [y]
-    | [x'] -> x::[x'], [y]
+    | [x'] -> x::y, [x']
     | _ -> let l1, l2 = split l in
            x::l1, y::l2
-
+(*)
 (* Verification succeeds even without this invariant;
    it just takes a lot longer (22s vs 7s) *)
 type merge_inv (l1:list int) (l2:list int) (l:list int) =
@@ -27,14 +94,18 @@ type merge_inv (l1:list int) (l2:list int) (l:list int) =
 val merge: l1:list int -> l2:list int -> Pure (list int)
              (requires (sorted l1 /\ sorted l2))
              (ensures (fun l -> sorted l /\ permutation_2 l l1 l2
-                                         /\ merge_inv l1 l2 l))
+                                         /\ merge_inv l1 l2 l
+                                         /\ (forall x y. ((appears_before x y l1 ==>
+                                          appears_before x y l)
+                                          /\(appears_before x y l2 ==>
+                                          appears_before x y l)))))
 let rec merge l1 l2 = match (l1, l2) with
   | [], _ -> l2
   | _, [] -> l1
   | h1::tl1, h2::tl2 -> if h1 <= h2
                         then h1::(merge tl1 l2)
                         else h2::(merge l1 tl2)
-
+(*)
 val mergesort: l:list int -> Pure (list int) (requires True)
       (ensures (fun r -> sorted r /\ permutation l r)) (decreases (length l))
 let rec mergesort l = match l with
