GenericSort.fst
@@ -1,0 +1,70 @@
+(**
+  @summary: This module defines properties of sortedness on a generic list.
+  @author: A Manning
+**)
+module GenericSort
+open FStar.List.Tot
+
+(**
+  key is a function that will appear a lot here,
+  as will 'a, a, #a, which are generic types.
+  key is a function on 'a that returns an integer.
+  #a and a appears where a is required to support equality.
+**)
+
+
+(**
+  Checks that a list is sorted.
+**)
+
+val appears_before: #a:eqtype -> before:a -> after:a -> ls: list a -> Tot bool
+let rec appears_before #a b4 aft ls =
+  match ls with
+  | _ | [_] -> false
+  | hd::tl ->
+    if hd = b4 then mem aft tl
+    else appears_before b4 aft tl
+
+type sort (#a:eqtype) (f:(list a -> k:(a -> Tot int) -> Tot (list a))) =
+  forall x y k zs. (mem x zs <==> mem x (f zs k)
+    /\ length zs = length (f zs k)
+    /\ (k x <= k y /\ mem x zs /\ mem y zs) <==> appears_before x y (f zs k))
+
+val sorted: list 'a -> key:('a -> Tot int) -> Tot bool
+let rec sorted l key = match l with
+    | [] | [_] -> true
+    | x::y::xs -> (key x <= key y) && (sorted (y::xs) key)
+
+val test_sorted: x:'a -> l:list 'a -> key:('a -> Tot int) ->
+      Lemma ((sorted (x::l) key /\ is_Cons l) ==> key x <= key (Cons.hd l))
+let test_sorted x l key = ()
+
+val test_sorted2: unit -> key:('a -> Tot int) -> Tot (m:list 'a{sorted m key})
+let test_sorted2 () key = Nil
+
+(**
+  Lemmata about sorted.
+**)
+val sorted_smaller: #a:eqtype
+                ->  x:a
+                ->  y:a
+                ->  l:list a
+                ->  key:(a -> Tot int)
+                ->  Lemma (requires (sorted (x::l) key /\ mem y l))
+                          (ensures (key x <= key y))
+                          [SMTPat (sorted (x::l) key); SMTPat (mem y l)]
+let rec sorted_smaller #a x y l key = match l with
+    | [] -> ()
+    | z::zs -> if key z = key y then () else sorted_smaller x y zs key
+
+val cons_sorted: #a:eqtype -> x:a -> l:list a{is_Cons l} -> key:(a -> Tot int)
+  -> Lemma(requires sorted l key /\ key x <= key (hd l))
+          (ensures sorted (x::l) key)
+let cons_sorted #a x l key = ()
+
+type permutation (#a:Type{hasEq a}) (l1:list a) (l2:list a) =
+    length l1 = length l2 /\ (forall n. mem n l1 = mem n l2)
+
+type permutation_2 (#a:Type{hasEq a}) (l:list a) (l1:list a) (l2:list a) =
+    (forall n. mem n l = (mem n l1 || mem n l2)) /\
+    length l = length l1 + length l2
