GenericStability.fst
@@ -1,0 +1,44 @@
+(**
+  @summary: This module defines sorting stability on the integers.
+  @author: A Manning
+**)
+module GenericStability
+open FStar.List.Tot
+open FStar.ListProperties
+open GenericSort
+(*
+  This module is heavily inspired by Leino and Lucio's 2012 paper,
+  'An Assertional Proof of the Stability and Correctness of Natural Mergesort'.
+  http://research.microsoft.com/en-us/um/people/leino/papers/krml241.pdf
+*)
+
+type stable (#a:eqtype) (l1:list a) (l2:list a{permutation l1 l2}) (key:(a -> Tot int)) =
+  forall x y. ((appears_before x y l1 /\ key y = key x) ==> appears_before x y l2)
+
+(**
+  filterEq returns the elements of a list that have the same key as n.
+**)
+val filter_eq: #a:Type -> (k:int) -> key:(a -> Tot int) -> (xs: list a) -> Tot (list a)
+let rec filter_eq #a k key xs =
+  match xs with
+  | [] -> []
+  | hd::tl
+    -> if key hd = k then
+        hd::(filter_eq k key tl)
+      else filter_eq k key tl
+
+val filter_eq_contains: #a:eqtype -> (k:int) -> key:(a -> Tot int) -> (xs: list a) ->
+  Lemma(ensures(forall x. (mem x xs /\ key x = k) <==> mem x (filter_eq k key xs)))
+let rec filter_eq_contains #a k key xs =
+  match xs with
+  | [] -> ()
+  | hd::tl ->
+    if key hd = k then
+      filter_eq_contains k key tl
+    else filter_eq_contains k key tl
+
+(*)
+val filter_eq_ordered: #a:eqtype -> key:(a -> Tot int) -> (xs: list a) ->
+  Lemma(ensures(forall x. ( (Cons.hd xs <> x)  /\ mem x (Cons.tl xs) /\ key (Cons.hd xs) = key x) ==>
+  (Cons.hd xs = Cons.hd (filter_eq (key x) key xs) /\ mem x (Cons.tl (filter_eq (key x) key xs)))))
+let filter_eq_ordered #a (key) xs = ()
